> [!note]
> Následující matice je preview pro Latex
>
$$\left( \begin{array}{cc} 2\tau & 7\phi-frac5{12} \\ 3\psi & \frac{\pi}8 \end{array} \right) \left( \begin{array}{c} x \\ y \end{array} \right) \mbox{~and~} \left[ \begin{array}{cc|r} 3 & 4 & 5 \\ 1 & 3 & 729 \end{array} \right]$$

$$A=\left[\begin{array}{cc} a & b  \\ c & d \end{array} \right]$$
$$\left[\begin{array}{cc} a & b  \\ c & d \end{array} \right]*\left[\begin{array}{cc} x & y  \\ z & t \end{array} \right] = \left[\begin{array}{cc} 1 & 0  \\ 0 & 1 \end{array} \right]$$
$$A^{-1} = \left[\begin{array}{cc} a & b  \\ c & d \end{array} \right]$$

Argumentovaná matice
$$A^*=A_{ij}^T$$
> [!missing]
> $${~když~} |A| \neq 0, {~tak~ A}$$ 


$$ A^{-1}=\frac{A*}{|A|} $$
$$|A^{-1}|=\frac{1}{|A|}; |A|\neq 0 $$

$$ (A*B)^{-1} = B^{-1}A^{-1}$$
$$(A^{-1})^T = (A^T)^{-1}$$

$$\left( \begin{array}{ccc} a_{11} & a_{12} & a_{13} \\ a_{21} & a_{22} & a_{23} \\ a_{31} & a_{32} & a_{33}\end{array} \right) * \left( \begin{array}{c} x \\ y \\ z \end{array} \right) = \left( \begin{array}{c} b_{1} \\ b_{2} \\ b_{3} \end{array} \right)$$
$$ \bar{x} = A^{-1}*b $$